strandspacegeneric.v
@@ -1,0 +1,328 @@
+
+Require Import Logic List ListSet Arith Peano_dec Omega Ensembles.
+Require Import Finite_sets_facts Finite_sets Relation_Definitions.
+Require Import Relation_Operators.
+Require Import strictorder set_rep_equiv util.
+Require Import finite_set_builder.
+
+Require Import strandspace.
+
+Section SimpleSpaces.
+
+Hypothesis PModel : PenetratorModel = DolevYao.
+
+Open Scope list_scope.
+Import ListNotations.
+Open Scope ss_scope.
+
+(* Proposition 3.3 
+   "Let C be a bundle, and let k be a Key s.t. ~ k in Kp,
+   If k never originates on a regular node, then K is not
+   a subterm of term(n) for any node n in C. In particular,
+   for any penetrator node p in C, k is not a subterm
+   of the term of p." *)
+Theorem non_origin_imp_non_subterm : forall B k,
+~ set_In k PKeys ->
+(forall n, Origin (#k) n -> ~ RegularNode n) ->
+(forall n, In Node (Nodes B) n -> ~ (#k) <st msg(n)).
+Proof.
+  intros B k notInKp noOrigin n nInN st.
+  remember B as bundle.
+  destruct bundle as [N E finN finE valE uniqtx acyc]; simpl in *.
+  assert (N = Nodes B) as NB. subst B. simpl; reflexivity.
+  clear Heqbundle.
+  assert (forall x : Node, {(#k) <st msg x} + {~ (#k) <st msg x})
+         as Pdec.
+    intros x. apply st_dec.    
+  destruct (ex_filter_ensemble 
+              Node 
+              eq_node_dec 
+              (fun n => (#k) <st (msg n)) 
+              Pdec
+              N 
+              finN) 
+    as [N' [inclN' N'memP]].
+  assert (Finite Node N') as finN'. eapply Finite_downward_closed.
+    exact finN. exact inclN'.
+  destruct finN' as [| N' fin x].
+  Case "Empty_set".
+    assert (In Node (Empty_set Node) n) as  contra.
+      apply N'memP. split. exact nInN. exact st.
+    inversion contra.
+  Case "non-empty".
+    assert (exists min, set_minimal (Add Node N' x) min) as exmin.
+      eapply (bundle_subset_minimal B). rewrite <- NB. exact inclN'.
+      intros contra. apply Add_not_Empty in contra. contradiction.
+    destruct exmin as [min minP].
+    assert (Origin (#k) min) as minorg.
+      eapply (min_origin B (Add Node N' x)). split.
+      intros [mIn mst].
+      apply N'memP. split. rewrite NB. exact mIn. exact mst.
+      intros mIn. split.
+      apply inclN' in mIn. rewrite <- NB. exact mIn.
+      apply N'memP in mIn. destruct mIn; auto. exact minP.
+    destruct (align_dec (strand min)) as [reg | pen].
+    eapply noOrigin. exact minorg. exact reg.
+    destruct minorg as [istx [minst minpred]].
+    assert (DolevYao (strand min)) as dymin.
+    rewrite <- PModel. apply penetrator_behavior. exact pen.
+    inversion dymin as 
+      [s t tunk seq minstrand | 
+       s g seq minstrand |
+       s g seq minstrand |
+       s g h seq minstrand |
+       s g h seq minstrand |
+       s k' kunk seq minstrand |
+       s h k' seq minstrand |
+      s h k' k'' inv seq minstrand]. 
+    SCase "M".
+      assert (length (strand min) = 1) as len. rewrite seq. auto.
+      assert ((index min) = 0) as imin. 
+        remember (index_len_node min). omega. 
+      assert (nth_error (strand min) (index min) = Some (smsg min)) as ntheq. 
+      apply node_indexing_equiv. 
+      rewrite seq in ntheq. rewrite imin in ntheq. simpl in ntheq.
+      inversion ntheq as [msmsg]. 
+      assert (msg min = (!t)) as minmsg.
+      apply node_smsg_msg_tx; auto. rewrite minmsg in minst. 
+      inversion minst.
+    SCase "F".
+      assert (length (strand min) = 1) as len. rewrite seq. auto.
+      assert ((index min) = 0) as imin. remember (index_len_node min); omega.
+      assert (nth_error (strand min) (index min) = Some (smsg min)) as ntheq. 
+      apply node_indexing_equiv. 
+      rewrite seq in ntheq. rewrite imin in ntheq. simpl in ntheq.
+      destruct istx as [t mmsg]. rewrite mmsg in ntheq.
+      inversion ntheq.
+    SCase "T".
+      assert (length (strand min) = 3) as len. rewrite seq. auto.
+      assert ((index min) = 0 
+              \/ (index min) = 1 
+              \/ (index min) = 2) as imin. remember (index_len_node min); omega.
+      assert (nth_error (strand min) (index min) = Some (smsg min)) as ntheq. 
+      apply node_indexing_equiv. 
+      destruct imin as [imin | irest].
+      SSCase "index min = 0".
+        rewrite seq in ntheq. rewrite imin in ntheq. simpl in ntheq.
+        inversion ntheq as [mmsg]. destruct istx as [t mtx]. 
+        rewrite mtx in mmsg.
+        inversion mmsg.
+      destruct irest as [imin | imin].
+      SSCase "index min = 1".
+        rewrite seq in ntheq. rewrite imin in ntheq. simpl in ntheq.
+        inversion ntheq as [mintxmsg]. 
+        assert (msg min = g) as minmsg.
+        apply node_smsg_msg_tx; auto. rewrite minmsg in minst.
+        destruct (strand_node (strand min) 0) as [y [ys yi]].
+          rewrite seq. simpl; auto. 
+        assert (y << min) as ypremin. constructor.
+          constructor 2. constructor. rewrite ys. reflexivity.
+          omega.
+        apply minpred in ypremin.
+        assert (nth_error (strand min) (index y) = Some (smsg y)) as ntheq2.
+          rewrite <- ys.
+        apply node_indexing_equiv. rewrite seq in ntheq2. rewrite yi in ntheq2.
+        simpl in ntheq2. inversion ntheq2 as [rxmsg]. symmetry in rxmsg. 
+        eapply node_smsg_msg_rx in rxmsg. rewrite rxmsg in ypremin.
+        contradiction.
+      SSCase "index min = 2".
+        rewrite seq in ntheq. rewrite imin in ntheq. simpl in ntheq.
+        inversion ntheq as [mintx]. 
+        assert (msg min = g) as minmsg.
+        apply node_smsg_msg_tx; auto. rewrite minmsg in minst.
+        destruct (strand_node (strand min) 1) as [y [ys yi]].
+          rewrite seq. simpl; auto. 
+        assert (y << min) as ypremin. constructor.
+          constructor 2. constructor. rewrite ys. reflexivity.
+          omega.
+        apply minpred in ypremin.
+        assert (nth_error (strand min) (index y) = Some (smsg y)) as ntheq2.
+          rewrite <- ys.
+        apply node_indexing_equiv. rewrite seq in ntheq2. rewrite yi in ntheq2.
+        simpl in ntheq2. inversion ntheq2 as [rxmsg]. symmetry in rxmsg. 
+        eapply node_smsg_msg_tx in rxmsg. rewrite rxmsg in ypremin.
+        contradiction.      
+    SCase "C".
+      assert (length (strand min) = 3) as len. rewrite seq. auto.
+      assert ((index min) = 0 
+              \/ (index min) = 1 
+              \/ (index min) = 2) as imin. remember (index_len_node min); omega.
+      assert (nth_error (strand min) (index min) = Some (smsg min)) as ntheq. 
+      apply node_indexing_equiv. 
+      destruct imin as [imin | irest].
+      SSCase "index min = 0".
+        rewrite seq in ntheq. rewrite imin in ntheq. simpl in ntheq.
+        destruct istx as [t mtx]. rewrite mtx in ntheq.
+        inversion ntheq.
+      destruct irest as [imin | imin].
+      SSCase "index min = 1".
+        rewrite seq in ntheq. rewrite imin in ntheq. simpl in ntheq.
+        destruct istx as [t mtx]. rewrite mtx in ntheq.
+        inversion ntheq.
+      SSCase "index min = 2".
+        destruct (strand_node (strand min) 0) as [n0 [n0s n0i]].
+          rewrite seq. simpl; auto. 
+        destruct (strand_node (strand min) 1) as [n1 [n1s n1i]].
+          rewrite seq. simpl; auto. 
+        rewrite seq in ntheq. rewrite imin in ntheq. simpl in ntheq.
+        inversion ntheq as [mmsg]. symmetry in mmsg. 
+        apply node_smsg_msg_tx in mmsg. rewrite mmsg in minst.
+        inversion minst as [m | m l r Hst | m l r Hst | m1 m2 k1 Hst]; subst.
+        SSSCase "#k <st g".
+          assert (n0 << min) as n0pred. econstructor 2. constructor. 
+            constructor 2. constructor. rewrite n0s. symmetry in n1s. 
+            exact n1s. omega. constructor. constructor 2. constructor. 
+            exact n1s. omega.
+          apply minpred in n0pred. 
+          assert (nth_error (strand n0) (index n0) = Some (smsg n0)) as ntheq2. 
+            apply node_indexing_equiv.
+          rewrite n0i in ntheq2. rewrite n0s in ntheq2. rewrite seq in ntheq2.
+          simpl in ntheq2. inversion ntheq2 as [rxmsg]. symmetry in rxmsg.
+          apply node_smsg_msg_rx in rxmsg. rewrite rxmsg in n0pred.
+          contradiction.
+        SSSCase "#k <st h".
+          assert (n1 << min) as n1pred. econstructor. constructor 2. 
+            constructor. auto. omega.
+          apply minpred in n1pred.
+          assert (nth_error (strand n1) (index n1) = Some (smsg n1)) as ntheq2. 
+            apply node_indexing_equiv.
+          rewrite n1s in ntheq2. rewrite n1i in ntheq2. rewrite seq in ntheq2.
+          simpl in ntheq2. inversion ntheq2 as [rxmsg]. symmetry in rxmsg.
+          apply node_smsg_msg_rx in rxmsg.
+          rewrite rxmsg in n1pred. contradiction.
+    SCase "S".
+      assert (length (strand min) = 3) as len. rewrite seq. auto.
+      assert ((index min) = 0 
+              \/ (index min) = 1 
+              \/ (index min) = 2) as imin. remember (index_len_node min); omega.
+      assert (nth_error (strand min) (index min) = Some (smsg min)) as ntheq. 
+      apply node_indexing_equiv. 
+      destruct imin as [imin | irest].
+      SSCase "index min = 0".
+        rewrite seq in ntheq. rewrite imin in ntheq. simpl in ntheq.
+        destruct istx as [t mtx]. rewrite mtx in ntheq.
+        inversion ntheq.
+      destruct irest as [imin | imin].
+      SSCase "index min = 1".
+        rewrite seq in ntheq. rewrite imin in ntheq. simpl in ntheq.
+        destruct (strand_node (strand min) 0) as [n0 [n0s n0i]].
+          rewrite seq. simpl; auto. 
+        assert (n0 << min) as n0pred. econstructor. constructor 2. 
+          constructor. auto. omega.
+        apply minpred in n0pred.
+        assert (nth_error (strand n0) (index n0) = Some (smsg n0)) as ntheq2.  
+          apply node_indexing_equiv.
+        rewrite n0s in ntheq2. rewrite n0i in ntheq2. rewrite seq in ntheq2.
+        simpl in ntheq2. inversion ntheq2 as [mrx]. symmetry in mrx.
+        apply node_smsg_msg_rx in mrx. rewrite mrx in n0pred.
+        assert (nth_error (strand min) (index min) = Some (smsg min)) as ntheq3. 
+          apply node_indexing_equiv.
+         rewrite seq in ntheq3. rewrite imin in ntheq3. simpl in ntheq3.
+         inversion ntheq3 as [mmsg]. symmetry in mmsg. 
+         apply node_smsg_msg_tx in mmsg.
+         rewrite mmsg in minst.
+         apply n0pred. constructor. exact minst.
+      SSCase "index min = 2".
+        rewrite imin in ntheq. rewrite seq in ntheq. simpl in ntheq.
+        destruct (strand_node (strand min) 0) as [n0 [n0s n0i]].
+          rewrite seq. simpl; auto. 
+        destruct (strand_node (strand min) 1) as [n1 [n1s n1i]].
+          rewrite seq. simpl; auto. 
+        assert (n0 << min) as n0pred. apply (t_trans Node SSEdge n0 n1 min). 
+          constructor. constructor 2. constructor. rewrite n0s. 
+          auto. omega. constructor. constructor 2. constructor.
+          exact n1s. omega.
+        apply minpred in n0pred.
+        assert (nth_error (strand n0) (index n0) = Some (smsg n0)) as ntheq2. 
+          apply node_indexing_equiv.
+        rewrite n0s in ntheq2. rewrite n0i in ntheq2. rewrite seq in ntheq2.
+        simpl in ntheq2. inversion ntheq2 as [mrx]. symmetry in mrx.
+        apply node_smsg_msg_rx in mrx. rewrite mrx in n0pred.
+        assert (nth_error (strand min) (index min) = Some (smsg min)) as ntheq3. 
+          apply node_indexing_equiv.
+         rewrite seq in ntheq3. rewrite imin in ntheq3. simpl in ntheq3.
+         inversion ntheq3 as [mtx]. symmetry in mtx. 
+         apply node_smsg_msg_tx in mtx.
+         rewrite mtx in minst.
+         apply n0pred. constructor 3. exact minst.
+    SCase "K".
+      destruct (eq_key_dec k k'); subst. contradiction.
+      assert (nth_error (strand min) (index min) = Some (smsg min)) as ntheq. 
+        apply node_indexing_equiv.
+      rewrite seq in ntheq. 
+      assert (length (strand min) = 1) as len. rewrite seq. auto.
+      assert ((index min) = 0)as imin. remember (index_len_node min); omega.
+      assert (nth_error (strand min) (index min) = Some (smsg min)) as ntheq2. 
+        apply node_indexing_equiv.
+      rewrite imin in ntheq2. rewrite seq in ntheq2. simpl in ntheq2.
+      inversion ntheq2 as [mtx]. symmetry in mtx. apply node_smsg_msg_tx in mtx.
+      rewrite mtx in minst.
+      inversion minst. contradiction.      
+    SCase "E".
+      assert (length (strand min) = 3) as len. rewrite seq. auto.
+      assert ((index min) = 0 
+              \/ (index min) = 1 
+              \/ (index min) = 2) as imin. remember (index_len_node min); omega.
+      assert (nth_error (strand min) (index min) = Some (smsg min)) as ntheq. 
+        apply node_indexing_equiv. 
+      destruct imin as [imin | irest].
+      SSCase "index min = 0".
+        rewrite imin in ntheq. rewrite seq in ntheq. simpl in ntheq.
+        inversion ntheq as [mrx]. destruct istx as [t mtx]. rewrite mtx in mrx.
+        inversion mrx.
+      destruct irest as [imin | imin].
+      SSCase "index min = 1".
+        rewrite imin in ntheq. rewrite seq in ntheq. simpl in ntheq.
+        inversion ntheq as [mrx]. destruct istx as [t mtx]. rewrite mtx in mrx.
+        inversion mrx.
+      SSCase "index min = 2".
+        rewrite imin in ntheq. rewrite seq in ntheq. simpl in ntheq.
+        inversion ntheq as [mtx]. symmetry in mtx. apply node_smsg_msg_tx in mtx.
+        rewrite mtx in minst.
+        inversion minst; subst.
+        destruct (strand_node (strand min) 1) as [n1 [n1s n1i]].
+          rewrite seq. simpl; auto.  
+        assert (n1 << min) as n1pre. constructor. constructor 2.
+          constructor. auto. omega.
+        apply minpred in n1pre.
+        assert (nth_error (strand n1) (index n1) = Some (smsg n1)) as ntheq2. 
+          apply node_indexing_equiv.        
+        rewrite n1i in ntheq2. rewrite seq in n1s. rewrite n1s in ntheq2. 
+        simpl in ntheq2. inversion ntheq2 as [mrx]. symmetry in mrx.
+        apply node_smsg_msg_rx in mrx. rewrite mrx in n1pre.
+        contradiction.
+    SCase "D".
+      assert (length (strand min) = 3) as len. rewrite seq. auto.
+      assert ((index min) = 0 
+              \/ (index min) = 1 
+              \/ (index min) = 2) as imin. remember (index_len_node min); omega.
+      assert (nth_error (strand min) (index min) = Some (smsg min)) as ntheq. 
+        apply node_indexing_equiv. 
+      destruct imin as [imin | irest].
+      SSCase "index min = 0".
+        rewrite imin in ntheq. rewrite seq in ntheq. simpl in ntheq.
+        inversion ntheq as [mrx]. symmetry in mrx.
+        destruct istx as [t mtx]. rewrite mtx in mrx. inversion mrx.
+      destruct irest as [imin | imin].
+      SSCase "index min = 1".
+        rewrite imin in ntheq. rewrite seq in ntheq. simpl in ntheq.
+        inversion ntheq as [mrx]. symmetry in mrx.
+        destruct istx as [t mtx]. rewrite mtx in mrx. inversion mrx.
+      SSCase "index min = 2".
+        destruct (strand_node (strand min) 1) as [n1 [n1s n1i]].
+          rewrite seq. simpl; auto.  
+        assert (n1 << min) as n1pre. constructor. constructor 2.
+          constructor. auto. omega.
+        apply minpred in n1pre.
+        assert (nth_error (strand n1) (index n1) = Some (smsg n1)) as ntheq2. 
+          apply node_indexing_equiv.        
+        rewrite n1s in ntheq2. rewrite seq in ntheq2. rewrite n1i in ntheq2. 
+        simpl in ntheq2. inversion ntheq2 as [mrx]. symmetry in mrx.
+        apply node_smsg_msg_rx in mrx. rewrite mrx in n1pre.
+        rewrite imin in ntheq. rewrite seq in ntheq. simpl in ntheq.
+        inversion ntheq as [mtx]. symmetry in mtx.
+        apply node_smsg_msg_tx in mtx. rewrite mtx in minst.
+        apply n1pre. constructor. exact minst.
+Qed.
+
+End SimpleSpaces.
